Add: new bytecode instructions

Exec.fst
@@ -10,12 +10,171 @@ let check_err dataStack =
     match (List.hd dataStack) with
     | ERR(s) -> Some (ERR(s))
     | _ -> None
-
+    
 (*
    Req: length(datastack) >= 1
 *)
 let return_value dataStack = List.hd dataStack
 
+(*
+   Req: length(datastack) >= 1
+*)
+let pop_top datastack = List.tail datastack
+
+(*
+   Req: length(datastack) >= 2
+*)
+let rot_two datastack = 
+  let fst_elem = List.hd datastack in
+  let scnd_elem = List.nth datastack 1 in
+  let _, rest_stack = List.splitAt 2 datastack in
+  scnd_elem::fst_elem::rest_stack
+
+(*
+   Req: length(datastack) >= 3
+*)
+let rot_three datastack = 
+  let fst_elem = List.hd datastack in
+  let scnd_elem = List.nth datastack 1 in
+  let thrd_elem = List.nth datastack 2 in
+  let _, rest_stack = List.splitAt 3 datastack in
+  scnd_elem::thrd_elem::fst_elem::rest_stack
+
+(*
+   Req: length(datastack) >= 4
+*)
+let rot_four datastack = 
+  let fst_elem = List.hd datastack in
+  let scnd_elem = List.nth datastack 1 in
+  let thrd_elem = List.nth datastack 2 in
+  let frth_elem = List.nth datastack 3 in
+  let _, rest_stack = List.splitAt 4 datastack in
+  scnd_elem::thrd_elem::frth_elem::fst_elem::rest_stack
+
+(*
+   Req: length(datastack) >= 1
+*)
+let dup_top datastack = 
+  let fst_elem = List.hd datastack in
+  fst_elem::datastack
+
+(*
+   Req: length(datastack) >= 2
+*)
+let dup_top_two datastack = 
+  let fst_elem = List.hd datastack in
+  let scnd_elem = List.nth datastack 1 in
+  fst_elem::scnd_elem::datastack
+
+
+(*
+   Req: length(datastack) >= 1
+*)
+let unary_positive datastack = 
+  let tos = List.hd datastack in
+  let newDataStack = List.tail datastack in
+  match tos with
+  | INT i -> INT(i)::newDataStack
+  | BOOL b -> INT(if b then 1 else 0)::newDataStack
+  | _ -> ERR("Error: bad operand type for unary +")::newDataStack
+
+(*
+   Req: length(datastack) >= 1
+*)
+let unary_negative datastack = 
+  let tos = List.hd datastack in
+  let newDataStack = List.tail datastack in
+  match tos with
+  | INT i -> INT(-i)::newDataStack
+  | BOOL b -> INT(if b then -1 else 0)::newDataStack
+  | _ -> ERR("Error: bad operand type for unary -")::newDataStack
+
+(*
+   Req: length(datastack) >= 1
+*)
+let unary_not datastack = 
+  let tos = List.hd datastack in
+  let newDataStack = List.tail datastack in
+  match tos with
+  | INT i -> BOOL(if i=0 then true else false)::newDataStack
+  | STRING s -> BOOL(if s="" then true else false)::newDataStack
+  | BOOL b -> BOOL(if b then false else true)::newDataStack
+  | NONE -> BOOL(true)::newDataStack
+  | _ -> ERR("Error: bad operand type for unary -")::newDataStack
+
+(*
+  Req: length(datastack) >= 2
+*)
+let binary_multiply (dataStack: list pyObj) = 
+  let tos = List.hd dataStack in
+  let tos1 = List.nth dataStack 1 in
+  let (_, newDataStack) = List.splitAt 2 dataStack in 
+  match (tos, tos1) with
+  | INT(i1), INT(i2) -> INT(op_Multiply i2 i1)::newDataStack
+  | BOOL(b1), BOOL(b2) -> INT(if b1&&b2 then 1 else 0)::newDataStack
+  | BOOL(b1), INT(i) -> INT(if b1 then i else  0)::newDataStack
+  | INT(i), BOOL(b2) -> INT(if b2 then i else 0)::newDataStack
+  | _, _ -> ERR("Error: unsupported operand type(s) for *")::newDataStack
+
+(*
+  Req: length(datastack) >= 2
+  ENS: (tos = tos1 // tos) or (tos = ERR)
+*)
+let binary_floor_divide (dataStack: list pyObj) = 
+  let tos = List.hd dataStack in
+  let tos1 = List.nth dataStack 1 in
+  let (_, newDataStack) = List.splitAt 2 dataStack in 
+  match (tos, tos1) with
+  | INT(a), INT(b) -> (if a=0 then ERR("Error: division by zero") else INT(b/a))::newDataStack
+  | BOOL(b1), BOOL(b2) -> (if not b1 then ERR("Error: division by zero") else if b2 then INT(1/1) else INT(0/1))::newDataStack
+  | INT(i), BOOL(b2) -> (if i=0 then ERR("Error: division by zero") else if b2 then INT(1/i) else INT(0/i))::newDataStack
+  | BOOL(b1), INT(i) -> (if not b1 then ERR("Error: division by zero") else INT(i/1))::newDataStack
+  | _, _ -> ERR("Error: unsupported operand type(s) for //")::newDataStack
+
+(*
+  Req: length(datastack) >= 2
+  ENS: (tos = tos1 % tos) or (tos = ERR)
+*)
+let binary_modulo (dataStack: list pyObj) = 
+  let tos = List.hd dataStack in
+  let tos1 = List.nth dataStack 1 in
+  let (_, newDataStack) = List.splitAt 2 dataStack in 
+  match (tos, tos1) with
+  | INT(a), INT(b) -> (if a=0 then ERR("Error: modulo by zero") else INT(b%a))::newDataStack
+  | BOOL(b1), BOOL(b2) -> (if not b1 then ERR("Error: modulo by zero") else if b2 then INT(1%1) else INT(0%1))::newDataStack
+  | INT(i), BOOL(b2) -> (if i=0 then ERR("Error: modulo by zero") else if b2 then INT(1%i) else INT(0%i))::newDataStack
+  | BOOL(b1), INT(i) -> (if not b1 then ERR("Error: modulo by zero") else INT(i%1))::newDataStack
+  | _, _ -> ERR("Error: unsupported operand type(s) for %")::newDataStack
+  
+(*
+  Req: length(datastack) >= 2
+*)
+let binary_add (dataStack: list pyObj) = 
+  let tos = List.hd dataStack in
+  let tos1 = List.nth dataStack 1 in
+  let (_, newDataStack) = List.splitAt 2 dataStack in 
+  match (tos, tos1) with
+  | INT(a), INT(b) -> INT(b + a)::newDataStack
+  | BOOL(b1), BOOL(b2) -> INT(if b1&&b2 then 2 else if b1||b2 then 1 else 0)::newDataStack
+  | BOOL(b1), INT(i) -> INT(if b1 then 1+i else  0+i)::newDataStack
+  | INT(i), BOOL(b2) -> INT(if b2 then 1+i else 0+i)::newDataStack
+  | STRING(s1), STRING(s2) -> STRING(s2 ^  s1)::newDataStack
+  | _, _ -> ERR("Error: unsupported operand type(s) for +")::newDataStack
+  
+(*
+  Req: length(datastack) >= 2
+*)
+let binary_subtract (dataStack: list pyObj) = 
+  let tos = List.hd dataStack in
+  let tos1 = List.nth dataStack 1 in
+  let (_, newDataStack) = List.splitAt 2 dataStack in 
+  match (tos, tos1) with
+  | INT(a), INT(b) -> INT(b - a)::newDataStack
+  | BOOL(b1), BOOL(b2) -> INT(if b1&&b2 then 0 else if b1 then -1 else if b2 then 1 else 0)::newDataStack
+  | BOOL(b1), INT(i) -> INT(if b1 then i-1 else  i-0)::newDataStack
+  | INT(i), BOOL(b2) -> INT(if b2 then 1+i else 0+i)::newDataStack
+  | _, _ -> ERR("Error: unsupported operand type(s) for -")::newDataStack
+  
 (*
   Req: (length(consts) > i) && (length(datastack) >= 1)
 *)
@@ -42,24 +201,113 @@ let store_fast i varnames dataStack =
   (newVarnames, newDataStack)
 
 (*
-  Req: length(datastack) >= 2
-*)
-let binary_add (dataStack: list pyObj) = 
-  let a = List.hd dataStack in
-  let b = List.nth dataStack 1 in
-  let (_, newDataStack) = List.splitAt 2 dataStack in 
-  match (a, b) with
-  | INT(a'), INT(b') -> INT(a' + b')::newDataStack
-  | STRING(a'), STRING(b') -> STRING(a' ^  b')::newDataStack
-  | _, _ -> ERR("Error: Adding two values of different types")::newDataStack
-
-(*
    Req: len(frame.fcode.bytecode) >= 1
 *)
 let rec execBytecode frame =
   let CODE(bc) = frame.fCode.co_code in
   match bc with
   | RETURN_VALUE::l -> return_value frame.dataStack
+
+  | NOP::l -> execBytecode ({frame with fCode = {frame.fCode with co_code = CODE l}})
+
+  | POP_TOP::l ->
+    let newDataStack = pop_top frame.dataStack in
+    let errCheck = check_err newDataStack in (
+    match errCheck with
+    | Some err -> err
+    | None -> execBytecode ({frame with dataStack = newDataStack; fCode = {frame.fCode with co_code = CODE l}}))
+  
+  | ROT_TWO::l ->
+    let newDataStack = rot_two frame.dataStack in
+    let errCheck = check_err newDataStack in (
+    match errCheck with
+    | Some err -> err
+    | None -> execBytecode ({frame with dataStack = newDataStack; fCode = {frame.fCode with co_code = CODE l}}))
+   
+  | ROT_THREE::l ->
+    let newDataStack = rot_three frame.dataStack in
+    let errCheck = check_err newDataStack in (
+    match errCheck with
+    | Some err -> err
+    | None -> execBytecode ({frame with dataStack = newDataStack; fCode = {frame.fCode with co_code = CODE l}}))
+   
+  | ROT_FOUR::l ->
+    let newDataStack = rot_four frame.dataStack in
+    let errCheck = check_err newDataStack in (
+    match errCheck with
+    | Some err -> err
+    | None -> execBytecode ({frame with dataStack = newDataStack; fCode = {frame.fCode with co_code = CODE l}}))
+
+  | DUP_TOP::l ->
+    let newDataStack = dup_top frame.dataStack in
+    let errCheck = check_err newDataStack in (
+    match errCheck with
+    | Some err -> err
+    | None -> execBytecode ({frame with dataStack = newDataStack; fCode = {frame.fCode with co_code = CODE l}}))
+
+  | DUP_TOP_TWO::l ->
+    let newDataStack = dup_top_two frame.dataStack in
+    let errCheck = check_err newDataStack in (
+    match errCheck with
+    | Some err -> err
+    | None -> execBytecode ({frame with dataStack = newDataStack; fCode = {frame.fCode with co_code = CODE l}}))
+
+  | UNARY_POSITIVE::l ->
+    let newDataStack = unary_positive frame.dataStack in
+    let errCheck = check_err newDataStack in (
+    match errCheck with
+    | Some err -> err
+    | None -> execBytecode ({frame with dataStack = newDataStack; fCode = {frame.fCode with co_code = CODE l}}))
+
+  | UNARY_NEGATIVE::l ->
+    let newDataStack = unary_negative frame.dataStack in
+    let errCheck = check_err newDataStack in (
+    match errCheck with
+    | Some err -> err
+    | None -> execBytecode ({frame with dataStack = newDataStack; fCode = {frame.fCode with co_code = CODE l}}))
+
+  | UNARY_NOT::l ->
+    let newDataStack = unary_not frame.dataStack in
+    let errCheck = check_err newDataStack in (
+    match errCheck with
+    | Some err -> err
+    | None -> execBytecode ({frame with dataStack = newDataStack; fCode = {frame.fCode with co_code = CODE l}}))
+
+  | BINARY_MULTIPLY::l -> 
+    let newDataStack = binary_multiply (frame.dataStack) in
+    let errCheck = check_err newDataStack in (
+    match errCheck with
+    | Some err -> err
+    | None -> execBytecode ({frame with dataStack = newDataStack; fCode = {frame.fCode with co_code = CODE l}}))
+    
+  | BINARY_FLOOR_DIVIDE::l -> 
+    let newDataStack = binary_floor_divide (frame.dataStack) in
+    let errCheck = check_err newDataStack in (
+    match errCheck with
+    | Some err -> err
+    | None -> execBytecode ({frame with dataStack = newDataStack; fCode = {frame.fCode with co_code = CODE l}}))    
+
+  | BINARY_MODULO::l -> 
+    let newDataStack = binary_modulo (frame.dataStack) in
+    let errCheck = check_err newDataStack in (
+    match errCheck with
+    | Some err -> err
+    | None -> execBytecode ({frame with dataStack = newDataStack; fCode = {frame.fCode with co_code = CODE l}}))
+    
+  | BINARY_ADD::l -> 
+    let newDataStack = binary_add (frame.dataStack) in
+    let errCheck = check_err newDataStack in (
+    match errCheck with
+    | Some err -> err
+    | None -> execBytecode ({frame with dataStack = newDataStack; fCode = {frame.fCode with co_code = CODE l}}))    
+
+  | BINARY_SUBTRACT::l -> 
+    let newDataStack = binary_subtract (frame.dataStack) in
+    let errCheck = check_err newDataStack in (
+    match errCheck with
+    | Some err -> err
+    | None -> execBytecode ({frame with dataStack = newDataStack; fCode = {frame.fCode with co_code = CODE l}})) 
+    
   | LOAD_CONST(i)::l ->
     let newDataStack = load_const i (frame.fCode.co_consts) (frame.dataStack) in
     let errCheck = check_err newDataStack in (
@@ -82,12 +330,5 @@ let rec execBytecode frame =
     | Some err -> err
     | None -> execBytecode ({frame with dataStack = newDataStack; fCode = newFCode}))
     
-  | BINARY_ADD::l -> 
-    let newDataStack = binary_add (frame.dataStack) in
-    let errCheck = check_err newDataStack in (
-    match errCheck with
-    | Some err -> err
-    | None -> execBytecode ({frame with dataStack = newDataStack; fCode = {frame.fCode with co_code = CODE l}}))
-    
-  | [] -> All.failwith "Error: reached empty bytecode array "
+    | [] -> All.failwith "Error: reached empty bytecode array "
 
