Exec.fsti
@@ -8,12 +8,38 @@ val check_err: list pyObj -> All.ML (option pyObj)
 
 val return_value: list pyObj -> All.ML pyObj
 
+val pop_top: list pyObj -> All.ML (list pyObj)
+
+val rot_two: list pyObj -> All.ML (list pyObj)
+
+val rot_three: list pyObj -> All.ML (list pyObj)
+
+val rot_four: list pyObj -> All.ML (list pyObj)
+
+val dup_top: list pyObj -> All.ML (list pyObj)
+
+val dup_top_two: list pyObj -> All.ML (list pyObj)
+
+val unary_positive: list pyObj -> All.ML (list pyObj)
+
+val unary_negative: list pyObj -> All.ML (list pyObj)
+
+val unary_not: list pyObj -> All.ML (list pyObj)
+
+val binary_multiply: list pyObj -> All.ML (list pyObj)
+
+val binary_floor_divide: list pyObj -> All.ML (list pyObj)
+
+val binary_modulo: list pyObj -> All.ML (list pyObj)
+
+val binary_add: list pyObj -> All.ML (list pyObj)
+
+val binary_subtract: list pyObj -> All.ML (list pyObj)
+
 val load_const: nat -> list pyObj -> list pyObj -> All.ML (list pyObj)
 
 val load_fast: nat -> list pyObj -> list pyObj -> All.ML (list pyObj)
 
 val store_fast: nat -> list pyObj -> list pyObj -> All.ML (list pyObj * list pyObj)
-
-val binary_add: list pyObj -> All.ML (list pyObj)
 
 val execBytecode: frameObj -> All.ML pyObj
