Utils.fst
@@ -9,5 +9,7 @@ let print_pyObj p =
   match p with
   | INT i -> Printf.sprintf "INT: %d" i
   | STRING s -> Printf.sprintf "STRING: %s" s
+  | BOOL b ->  Printf.sprintf "BOOL: %b" b
   | NONE -> Printf.sprintf "NONE"
   | ERR s -> Printf.sprintf "ERR: %s" s
+  (*| _ -> Printf.sprintf ""*)
